fstar/Hacspec.Chacha20.fst
@@ -166,7 +166,6 @@ let chacha (key_1911 : key) (iv_1912 : iv) (m_1913 : byte_seq) : byte_seq =
   let blocks_out_1915 = seq_new_ (secret (pub_u8 0x8)) (seq_len (m_1913)) in
   let (ctr_1914, blocks_out_1915) =
     foldi
-      (**) #(_ & lseq uint8 (seq_len (m_1913)))
       (usize 0) (seq_num_chunks (m_1913) (usize 64)) (fun i_1916 (
         ctr_1914,
         blocks_out_1915
